Yet another statement of instantiate_params_subst_inst

pcuic/theories/PCUICSigmaCalculus.v
@@ -53,29 +53,105 @@ Proof.
     specialize (h _ _ e).
 Admitted.
 
+(* TODO DUPLICATE MOVE *)
+Definition on_pair {A B C D} (f : A -> B) (g : C -> D) (x : A * C) :=
+  (f (fst x), g (snd x)).
+
 Lemma instantiate_params_subst_inst :
-  forall params pars s ty σ s' T,
-    instantiate_params_subst params pars s ty = Some (s', T) ->
-    instantiate_params_subst params (map (inst σ) pars) (map (inst σ) s) ty =
-    Some (map (inst σ) s', T).
+  forall params pars s ty σ,
+    instantiate_params_subst
+      (mapi_rec (fun i decl => map_decl (inst (⇑^i σ)) decl) params #|s|)
+      (map (inst σ) pars)
+      (map (inst σ) s)
+      ty.[⇑^#|s| σ]
+    =
+    option_map
+      (on_pair (map (inst σ)) (inst (⇑^(#|s| + #|params|) σ)))
+      (instantiate_params_subst params pars s ty).
 Proof.
-  intros params pars s ty σ s' T e.
-  induction params in pars, s, ty, σ, s', T, e |- *.
-  - simpl in *. destruct pars ; try discriminate.
-    inversion e. subst. clear e.
-    simpl. reflexivity.
-  - simpl in *.
-    destruct (decl_body a).
-    + destruct ty. all: try discriminate e.
-      eapply IHparams with (σ := σ) in e as ih. simpl in ih.
-      rewrite <- ih. f_equal. f_equal.
-      autorewrite with sigma.
-      eapply inst_ext. intro i.
-      unfold subst_consn, subst_compose.
-      rewrite nth_error_map.
-      destruct (nth_error s i).
-      * simpl. reflexivity.
-      * simpl. give_up.
+  intros params pars s ty σ.
+  induction params in pars, s, ty, σ |- *.
+  - simpl. destruct pars. 2: reflexivity.
+    simpl. unfold on_pair. simpl. f_equal. f_equal. f_equal. f_equal. omega.
+  - simpl. destruct (decl_body a).
+    + simpl. destruct ty. all: try reflexivity.
+      * simpl. admit.
+      * simpl. specialize (IHparams pars ((subst0 s) t :: s)).
+        simpl in IHparams.
+        replace (#|s| + S #|params|)
+          with (S (#|s| + #|params|))
+          by omega.
+        rewrite <- IHparams. f_equal.
+        -- f_equal. autorewrite with sigma.
+           eapply inst_ext. intro i.
+           unfold Upn, subst_consn, subst_compose.
+
+Lemma nth_error_idsn_Some :
+  forall n k,
+    k < n ->
+    nth_error (idsn n) k = Some (tRel k).
+Proof.
+  intros n k h.
+  induction n in k, h |- *.
+  - inversion h.
+  - simpl. destruct (Nat.ltb_spec0 k n).
+    + rewrite nth_error_app1.
+      * rewrite idsn_length. auto.
+      * eapply IHn. assumption.
+    + assert (k = n) by omega. subst.
+      rewrite nth_error_app2.
+      * rewrite idsn_length. auto.
+      * rewrite idsn_length. replace (n - n) with 0 by omega.
+        simpl. reflexivity.
+Qed.
+
+           case_eq (nth_error s i).
+           ++ intros t' e.
+              rewrite nth_error_idsn_Some.
+              ** eapply nth_error_Some_length. eassumption.
+              ** simpl.
+                 rewrite nth_error_map. rewrite e. simpl.
+                 reflexivity.
+           ++ intro neq.
+
+Lemma nth_error_idsn_None :
+  forall n k,
+    k >= n ->
+    nth_error (idsn n) k = None.
+Proof.
+  intros n k h.
+  eapply nth_error_None.
+  rewrite idsn_length. auto.
+Qed.
+
+              rewrite nth_error_idsn_None.
+              ** eapply nth_error_None. assumption.
+              ** simpl. rewrite idsn_length.
+                 autorewrite with sigma.
+
+
+
+(*     instantiate_params_subst params pars s ty = Some (s', T) -> *)
+(*     instantiate_params_subst params (map (inst σ) pars) (map (inst σ) s) ty = *)
+(*     Some (map (inst σ) s', T). *)
+(* Proof. *)
+(*   intros params pars s ty σ s' T e. *)
+(*   induction params in pars, s, ty, σ, s', T, e |- *. *)
+(*   - simpl in *. destruct pars ; try discriminate. *)
+(*     inversion e. subst. clear e. *)
+(*     simpl. reflexivity. *)
+(*   - simpl in *. *)
+(*     destruct (decl_body a). *)
+(*     + destruct ty. all: try discriminate e. *)
+(*       eapply IHparams with (σ := σ) in e as ih. simpl in ih. *)
+(*       rewrite <- ih. f_equal. f_equal. *)
+(*       autorewrite with sigma. *)
+(*       eapply inst_ext. intro i. *)
+(*       unfold subst_consn, subst_compose. *)
+(*       rewrite nth_error_map. *)
+(*       destruct (nth_error s i). *)
+(*       * simpl. reflexivity. *)
+(*       * simpl. give_up. *)
 Abort.
 
 Lemma instantiate_params_inst :
