pcuic/theories/PCUICWeakening.v
@@ -475,6 +475,7 @@ Qed.
 (*   now rewrite IHt1. *)
 (* Qed. *)
 
+(* TODO DUPLICATE MOVE *)
 Definition on_pair {A B C D} (f : A -> B) (g : C -> D) (x : A * C) :=
   (f (fst x), g (snd x)).
 
